tests/DepDestruct.v
@@ -1,0 +1,202 @@
+From Coq Require Import List.
+Import ListNotations.
+From MetaCoq
+Require Export MetaCoq MCListUtils MCTactics ImportedTactics DepDestruct.
+Import MetaCoqNotations.
+Import MCTacticsNotations.
+
+Section ExampleReflect.
+
+  Inductive reflect (P :Prop) : bool -> Type :=
+  | RTrue : P -> reflect P true
+  | RFalse : ~P -> reflect P false.
+
+  Example reflect_reflect P : ITele (SType) := iTele (fun b=>@iBase SType (reflect P b)).
+
+  Example reflect_RTrue P : CTele (reflect_reflect P) :=
+    (cProd (fun p=>@cBase SType _ (aTele _ (aBase)) (RTrue P p))).
+
+  Example reflect_RFalse P : CTele (reflect_reflect P) :=
+    (cProd (fun p=>@cBase SType _ (aTele _ (aBase)) (RFalse P p))).
+
+  Example reflect_args P b : ATele (reflect_reflect P) :=
+    aTele b aBase.
+
+  Example bla P : RTele _ (reflect_reflect P) :=
+    Eval simpl in rTele (fun b=>rBase (rsort:=SProp) (fun _=>P <-> b = true)).
+  Example bla_branch P := Eval simpl in get_type_of_branch (bla P) (reflect_RTrue P).
+
+
+  Example bla_RTele P b (r : reflect P b) :=
+    Eval compute in eval (abstract_goal (rsort := SProp) (reflect_args P b) ((P <-> b = true)) r).
+
+  Example bla_goals P b r : list dyn :=
+    Eval compute in
+      map (fun cs => Dyn (get_type_of_branch (rsort := SProp) (bla_RTele P b r) cs))
+          (reflect_RTrue P :: reflect_RFalse P :: nil).
+
+  Example reflectP_it : ITele _ :=
+    iTele (fun P => iTele (fun b => iBase (sort := SType) (reflect P b))).
+  Program Example reflectP_RTrue : CTele reflectP_it :=
+    cProd (fun P => cProd (fun p => (cBase (aTele _ (aTele _ aBase)) (@RTrue P p)))).
+  Program Example reflectP_RFalse : CTele reflectP_it :=
+    cProd (fun P => cProd (fun np => (cBase (aTele _ (aTele _ aBase)) (@RFalse P np)))).
+  Example reflectP_args P b : ATele reflectP_it :=
+    aTele P (aTele b (aBase)).
+
+  Example reflect_app P b := Eval compute in ITele_App (reflect_args P b).
+
+  Example blaP_RTele P b r :=
+    Eval compute in eval (abstract_goal (rsort := SProp) (reflectP_args P b) ((P <-> b = true)) r).
+
+  Example blaP_goals P b r : list dyn :=
+    Eval compute in
+      map (fun cs => Dyn (get_type_of_branch (blaP_RTele P b r) cs))
+          (reflectP_RFalse :: reflectP_RTrue :: nil).
+
+  Goal True.
+    MProof.
+    (fun g =>
+       r <- destcase (match 3 with 0 => true | S _ => false end);
+       print_term r;;
+                  cpose r (fun r=>idtac) g) : tactic.
+    (fun g=>
+       case <- makecase r;
+       cpose case (fun y=>idtac) g) : tactic.
+  Abort.
+
+  Goal forall P b, reflect P b -> P <-> b = true.
+  Proof.
+    intros P b r.
+    pose (rG := eval (abstract_goal (rsort := SType) (reflect_args P b) (P <-> b = true) r)).
+    simpl in rG.
+    assert (T : get_type_of_branch rG (reflect_RTrue P)).
+    { now firstorder. }
+    assert (F : get_type_of_branch rG (reflect_RFalse P)).
+    { compute. firstorder. now discriminate. }
+    pose (mc :=
+            makecase {|
+                case_val := r;
+                case_type := RTele_App rG (reflect_args P b) r;
+                case_return := Dyn (RTele_Fun rG);
+                case_branches := (Dyn T) :: (Dyn F) :: nil
+              |}).
+    compute in mc.
+    pose (c := eval mc).
+    unfold eval in c.
+    exact (elem c).
+  Qed.
+
+Notation "'mpose' ( x := t )" := ((fun g=>r <- t; cpose r (fun x=>idtac) g) : tactic)
+  (at level 40, x at next level).
+
+Fixpoint unfold_funs {A} (t: A) (n: nat) {struct n} : M A :=
+  match n with
+  | 0 => ret t
+  | S n' =>
+    mmatch A as A' return M A' with
+    | [? B (fty : B -> Type)] forall x, fty x => [H]
+      let t' := match H in _ = P return P with eq_refl => t end in (* we need to reduce this *)
+      nu x,
+        r <- unfold_funs (t' x) n';
+      abs x r
+    | [? A'] A' => [H]
+      match H in _ = P return M P with eq_refl => ret t end
+    end
+  end.
+
+(* MetaCoq version *)
+Goal forall P b, reflect P b -> P <-> b = true.
+MProof.
+  intros P b r.
+  mpose (rG := abstract_goal (rsort := SType) (reflect_args P b) (P <-> b = true) r).
+  tsimpl.
+  assert (T : get_type_of_branch rG (reflect_RTrue P)).
+  - cintros x {- MCTactics.split;; [cintros P {- reflexivity -}; cintros notP {- assumption -}] -}. (* it doesn't work if intros is put outside *)
+  assert (F : get_type_of_branch rG (reflect_RFalse P)).
+  - tsimpl. intros. MCTactics.split. intros. exact (match a x with end). intros;; discriminate.
+  pose (mc :=
+          makecase {|
+              case_val := r;
+              case_type := RTele_App rG (reflect_args P b) r;
+              case_return := Dyn (typ2);
+              case_branches := (Dyn T) :: (Dyn F) :: nil
+            |}).
+  mpose (c := mc).
+  exact (elem c).
+Qed.
+
+
+End ExampleReflect.
+
+
+Module VectorExample.
+Require Import Vector.
+Goal forall n (v : t nat n), n = length (to_list v).
+Proof.
+  pose (it := iTele (fun n => @iBase (SType) (t nat n))).
+  pose (vnil := ((@cBase SType _ (aTele 0 aBase) (nil nat))) : CTele it).
+  pose (vcons := (cProd (fun a => cProd (fun n => cProd (fun (v : t nat n) => (@cBase SType _ (aTele (S n) aBase) (cons _ a _ v)))))) : CTele it).
+  fix f 2.
+  intros n v.
+  pose (a := (aTele n (aBase)) : ATele it).
+  pose (rt := eval (abstract_goal (rsort := SProp) a (n = length (to_list v)) v)).
+  simpl in vcons, rt.
+  assert (N : get_type_of_branch rt vnil).
+  { now auto. }
+  assert (C : get_type_of_branch rt vcons).
+  { intros x k v'. hnf. simpl. f_equal. exact (f _ _). }
+  pose (mc :=
+          makecase {|
+              case_val := v;
+              case_type := RTele_App rt a v;
+              case_return := Dyn (RTele_Fun rt);
+              case_branches := Dyn N :: Dyn C :: List.nil
+            |}
+       ).
+  simpl RTele_Fun in mc.
+  (* pose (ma := (match v as v' in t _ k return k = length (to_list v') with *)
+  (*              | nil _ => N *)
+  (*              | cons _ a k v => C a k v *)
+  (*              end)). *)
+  (* pose (c' := eval (destcase ma)). *)
+  (* unfold eval in c'. *)
+  pose (c := eval mc).
+  unfold eval in c.
+  exact (elem c).
+Qed.
+End VectorExample.
+
+
+Example get_reflect_ITele := Eval compute in ltac:(mrun (get_ITele (reflect True))).
+Example reflect_nindx := Eval compute in let (n, _) := get_reflect_ITele in n.
+Example reflect_sort := Eval compute in let (sort, _) := snd get_reflect_ITele in sort.
+Example reflect_itele : ITele reflect_sort :=
+  Eval compute in
+  match snd get_reflect_ITele as pair return let (sort, _) := pair in ITele sort with
+  | existT _ s it => it
+  end.
+
+Example args_of_RTrue P := Eval compute in ltac:(mrun (args_of _ (reflect P true))).
+Example args_of_max_RTrue P := Eval compute in ltac:(mrun (args_of_max 2 (reflect P true))).
+
+
+Example ATele_of_RTrue := Eval compute in ltac:(mrun (get_ATele (reflect_itele) (tail (args_of_RTrue True)))).
+
+Example get_RTrue_CTele := Eval compute in ltac:(mrun (get_CTele reflect_itele 1 _ (RTrue True))).
+Example get_RFalse_CTele := Eval compute in ltac:(mrun (get_CTele reflect_itele 1 _ (RFalse True))).
+
+
+
+
+
+Example test P b (r : reflect P b) : P -> if b then nat else True -> nat.
+MProof.
+  new_destruct r.
+  ltac:(
+    mrun ((fun g =>
+             t <- new_destruct r g;
+               print "debuggery";;
+               print_term t;;
+                          ret [g]) : tactic)
+).
